Symbols and fonts

NuPrime.thy
@@ -268,26 +268,26 @@ type_synonym assn = "(heap \<times> stack) set" \<comment> \<open>assertion\<clo
 
 subsubsection \<open>Types specifying states\<close>
 
-definition StrictStateTy :: " (heap \<times> 'a::lrep) set \<Rightarrow> 'a state set" ("\<S_S> _" [56] 55)
-  where "\<S_S> T = {s. case s of Success x \<Rightarrow> x \<in> T | Fail \<Rightarrow> False | PartialCorrect \<Rightarrow> False}"
+definition StrictStateTy :: " (heap \<times> 'a::lrep) set \<Rightarrow> 'a state set" ("!\<S> _" [56] 55)
+  where "!\<S> T = {s. case s of Success x \<Rightarrow> x \<in> T | Fail \<Rightarrow> False | PartialCorrect \<Rightarrow> False}"
 definition LooseStateTy :: " (heap \<times> 'a::lrep) set \<Rightarrow> 'a state set" ("\<S> _" [56] 55)
   where "\<S> T = {s. case s of Success x \<Rightarrow> x \<in> T | Fail \<Rightarrow> False | PartialCorrect \<Rightarrow> True}"
 
-lemma StrictStateTy_expn[iff,\<nu>def]: "Success x \<in> \<S_S> T \<equiv> x \<in> T"  "\<not> (Fail \<in> \<S_S> T)"  "\<not> (PartialCorrect \<in> \<S_S> T)"
+lemma StrictStateTy_expn[iff,\<nu>def]: "Success x \<in> !\<S> T \<equiv> x \<in> T"  "\<not> (Fail \<in> !\<S> T)"  "\<not> (PartialCorrect \<in> !\<S> T)"
   and LooseStateTy_expn[iff,\<nu>def]: "Success x \<in> \<S> T \<equiv> x \<in> T"  "\<not> (Fail \<in> \<S> T)"  "(PartialCorrect \<in> \<S> T)"
   by (simp_all add: StrictStateTy_def LooseStateTy_def)
 lemma LooseStateTy_expn' : "x \<in> \<S> T \<longleftrightarrow> x = PartialCorrect \<or> (\<exists>x'. x = Success x' \<and> x' \<in> T)"
   by (cases x) simp_all
 
-lemma StrictStateTy_elim[elim]: "s \<in> \<S_S> T \<Longrightarrow> (\<And>x. s = Success x \<Longrightarrow> x \<in> T \<Longrightarrow> C) \<Longrightarrow> C" by (cases s) auto
-lemma StrictStateTy_intro[intro]: " x \<in> T \<Longrightarrow> Success x \<in> \<S_S> T" by simp
+lemma StrictStateTy_elim[elim]: "s \<in> !\<S> T \<Longrightarrow> (\<And>x. s = Success x \<Longrightarrow> x \<in> T \<Longrightarrow> C) \<Longrightarrow> C" by (cases s) auto
+lemma StrictStateTy_intro[intro]: " x \<in> T \<Longrightarrow> Success x \<in> !\<S> T" by simp
 lemma LooseStateTy_E[elim]:
   "s \<in> \<S> T \<Longrightarrow> (\<And>x. s = Success x \<Longrightarrow> x \<in> T \<Longrightarrow> C) \<Longrightarrow> (s = PartialCorrect \<Longrightarrow> C) \<Longrightarrow> C" by (cases s) auto
 lemma LooseStateTy_I[intro]:
   " x \<in> T \<Longrightarrow> Success x \<in> \<S> T" and [intro]: "PartialCorrect \<in> \<S> T" by simp_all
-lemma LooseStateTy_upgrade: "s \<in> \<S> T \<Longrightarrow> s \<noteq> PartialCorrect \<Longrightarrow> s \<in> \<S_S> T" by (cases s) auto
-lemma StrictStateTy_degrade: "s \<in> \<S_S> T \<Longrightarrow> s \<in> \<S> T" by (cases s) auto
-lemma LooseStateTy_introByStrict: "(s \<noteq> PartialCorrect \<Longrightarrow> s \<in> \<S_S> T) \<Longrightarrow> s \<in> \<S> T" by (cases s) auto
+lemma LooseStateTy_upgrade: "s \<in> \<S> T \<Longrightarrow> s \<noteq> PartialCorrect \<Longrightarrow> s \<in> !\<S> T" by (cases s) auto
+lemma StrictStateTy_degrade: "s \<in> !\<S> T \<Longrightarrow> s \<in> \<S> T" by (cases s) auto
+lemma LooseStateTy_introByStrict: "(s \<noteq> PartialCorrect \<Longrightarrow> s \<in> !\<S> T) \<Longrightarrow> s \<in> \<S> T" by (cases s) auto
 
 subsubsection \<open>Shallow model and Deep model\<close>
 
@@ -491,7 +491,7 @@ subsubsection \<open>Construction Context & Code block\<close>
 
 definition CurrentConstruction :: " ('a::stack) state \<Rightarrow> assn \<Rightarrow> assn \<Rightarrow> bool "
     ("\<^bold>c\<^bold>u\<^bold>r\<^bold>r\<^bold>e\<^bold>n\<^bold>t _ [_] \<^bold>r\<^bold>e\<^bold>s\<^bold>u\<^bold>l\<^bold>t\<^bold>s \<^bold>i\<^bold>n/ _" [1000,1000,11] 10)
-  where "CurrentConstruction s R S \<longleftrightarrow> s \<in> \<S_S> Heap' (Shallowize' (R \<heavy_asterisk> S))"
+  where "CurrentConstruction s R S \<longleftrightarrow> s \<in> !\<S> Heap' (Shallowize' (R \<heavy_asterisk> S))"
 definition PendingConstruction :: " (('a::stack) \<longmapsto> ('b::stack)) \<Rightarrow> 'a state \<Rightarrow> assn \<Rightarrow> assn \<Rightarrow> bool "
     ("\<^bold>p\<^bold>e\<^bold>n\<^bold>d\<^bold>i\<^bold>n\<^bold>g _ \<^bold>o\<^bold>n _ [_] \<^bold>r\<^bold>e\<^bold>s\<^bold>u\<^bold>l\<^bold>t\<^bold>s \<^bold>i\<^bold>n/ _" [1000,1000,1000,5] 4)
   where "PendingConstruction f s R S \<longleftrightarrow> bind s f \<in> \<S> Heap' (Shallowize' (R \<heavy_asterisk> S))"
